Leanactors.lean
@@ -3,3 +3,4 @@ import Leanactors.Props
 import Leanactors.Count
 import Leanactors.Examples.Bank
 import Leanactors.Examples.Lock
+import Leanactors.Examples.LockProof
